trace-symexec/output.bpl
@@ -38,26 +38,93 @@ modifies balances;
     var _value: uint256;
     var _fee: uint256;
        
-	var tmp2: uint256;
 	var tmp1: uint256;
-	var tmp3: uint256;
-	var tmp4: uint256;
-	var tmp5: bool;
-	var tmp6: bool;
+	var tmp2: uint256;
+	var tmp3: bool;
+	var tmp4: bool;
+	var tmp6: uint256;
+	var tmp5: uint256;
+	var tmp7: uint256;
+	var tmp8: bool;
+	var tmp9: bool;
+	var tmp11: uint256;
+	var tmp12: uint256;
+	var tmp13: uint256;
+	var tmp14: bool;
+	var tmp15: bool;
+	var tmp10: uint256;
+	var tmp16: uint256;
+	var tmp17: bool;
+	var tmp18: bool;
+	var tmp20: uint256;
+	var tmp22: uint256;
+	var tmp21: uint256;
+	var tmp23: uint256;
+	var tmp24: bool;
+	var tmp25: bool;
+	var tmp19: uint256;
+	var tmp27: uint256;
+	var tmp29: uint256;
+	var tmp30: uint256;
+	var tmp31: uint256;
+	var tmp32: bool;
+	var tmp33: bool;
+	var tmp28: uint256;
+	var tmp34: uint256;
+	var tmp35: bool;
+	var tmp36: bool;
+	var tmp26: uint256;
 
     assume (0<=_value && _value<TwoE255+1 && 0<=_fee && _fee<TwoE255);           
     assume (totalSupply<TwoE255);    
 
     assume (sum(balances) == totalSupply);
     assume (forall x:address :: 0<=balances[x] && balances[x]<=totalSupply);  
-	tmp2:=evmand(1461501637330902918203684832716283019655932542975,_from);
-	tmp1:=evmand(1461501637330902918203684832716283019655932542975,tmp2);
-	tmp3:=balances[tmp1];
-	tmp4:=evmadd(_fee,_value);
-	tmp5:=tmp3<tmp4;
-	tmp6:=!tmp5;
-	assume(tmp6);
-	
+
+	tmp1:=mapID2[_from];
+	tmp2:=evmadd(_fee,_value);
+	tmp3:=tmp1<tmp2;
+	tmp4:=!tmp3;
+	assume(tmp4);
+
+	tmp6:=mapID2[_value];
+	tmp5:=evmadd(tmp6,_fee);
+	tmp7:=mapID2[_value];
+	tmp8:=tmp5<tmp7;
+	tmp9:=!tmp8;
+	assume(tmp9);
+
+	tmp11:=mapID2[msg.sender];
+	tmp12:=mapID2[_from];
+	tmp13:=evmadd(_fee,_value);
+	tmp14:=tmp12<tmp13;
+	tmp15:=!tmp14;
+	tmp10:=evmadd(tmp11,tmp15);
+	tmp16:=mapID2[msg.sender];
+	tmp17:=tmp10<tmp16;
+	tmp18:=!tmp17;
+	assume(tmp18);
+
+	tmp20:=mapID2[_from];
+	tmp22:=mapID2[_value];
+	tmp21:=evmadd(tmp22,_fee);
+	tmp23:=mapID2[_value];
+	tmp24:=tmp21<tmp23;
+	tmp25:=!tmp24;
+	tmp19:=evmadd(tmp20,tmp25);
+	mapID2[None]:=tmp19	tmp27:=mapID2[msg.sender];
+	tmp29:=mapID2[msg.sender];
+	tmp30:=mapID2[_from];
+	tmp31:=evmadd(_fee,_value);
+	tmp32:=tmp30<tmp31;
+	tmp33:=!tmp32;
+	tmp28:=evmadd(tmp29,tmp33);
+	tmp34:=mapID2[msg.sender];
+	tmp35:=tmp28<tmp34;
+	tmp36:=!tmp35;
+	tmp26:=evmadd(tmp27,tmp36);
+	mapID2[None]:=tmp26	mapID2[None]:=SUB(SLOAD(MapElement(2,0)),ADD(ISZERO(LT(ADD(SLOAD(MapElement(2,AND(1461501637330902918203684832716283019655932542975,AND(1461501637330902918203684832716283019655932542975,_value)))),_fee),SLOAD(MapElement(2,AND(1461501637330902918203684832716283019655932542975,AND(1461501637330902918203684832716283019655932542975,_value)))))),ISZERO(LT(ADD(SLOAD(MapElement(2,AND(1461501637330902918203684832716283019655932542975,AND(1461501637330902918203684832716283019655932542975,msg.sender)))),ISZERO(LT(SLOAD(MapElement(2,AND(1461501637330902918203684832716283019655932542975,AND(1461501637330902918203684832716283019655932542975,_from)))),ADD(_fee,_value)))),SLOAD(MapElement(2,AND(1461501637330902918203684832716283019655932542975,AND(1461501637330902918203684832716283019655932542975,msg.sender))))))))	
     assert (sum(balances) == totalSupply);         
     assert (forall x:address :: 0<=balances[x] && balances[x]<=totalSupply);
+
 }   
